theories/ml_toy_lang/logrel/iterup.v
@@ -1,0 +1,23 @@
+From iris.program_logic Require Import weakestpre.
+From iris.base_logic Require Import invariants.
+From Autosubst Require Export Autosubst.
+From iris.prelude Require Import options.
+
+Canonical Structure varO := leibnizO var.
+
+Section Autosubst_Lemmas.
+  Context {term : Type} {Ids_term : Ids term}
+          {Rename_term : Rename term} {Subst_term : Subst term}
+          {SubstLemmas_term : SubstLemmas term}.
+
+  Lemma iter_up (m x : nat) (f : var → term) :
+    upn m f x = if lt_dec x m then ids x else rename (+m) (f (x - m)).
+  Proof using Type*.
+    revert x; induction m as [|m IH]=> -[|x];
+      repeat (destruct (lt_dec _ _) || asimpl || rewrite IH); auto with lia.
+  Qed.
+End Autosubst_Lemmas.
+
+Reserved Notation "⟦ τ ⟧" (at level 0, τ at level 70).
+Reserved Notation "⟦ τ ⟧ₑ" (at level 0, τ at level 70).
+Reserved Notation "⟦ Γ ⟧*" (at level 0, Γ at level 70).
