theories/ml_toy_lang/logrel/logrel.v
@@ -1,0 +1,242 @@
+From iris.proofmode Require Import proofmode.
+From melocoton.ml_toy_lang.logrel Require Export persistent_pred typing iterup.
+From melocoton.ml_toy_lang.melocoton Require Export proofmode.
+From melocoton.ml_toy_lang Require Export lang notation metatheory.
+From iris.algebra Require Import list gmap big_op.
+From iris.base_logic Require Import invariants.
+From iris.prelude Require Import options.
+From melocoton.language Require Export weakestpre wp_link.
+From Autosubst Require Export Autosubst.
+Import uPred.
+
+Definition logN : namespace := nroot .@ "logN".
+
+(** interp : is a unary logical relation. *)
+Section logrel.
+  Context `{!heapGS_ML Σ, !invGS_gen hlc Σ}.
+  Notation D := (persistent_predO val (iPropI Σ)).
+  Implicit Types τi : D.
+  Implicit Types Δ : listO D.
+  Implicit Types interp : listO D -n> D.
+
+  Local Arguments ofe_car !_.
+
+
+  Context (T : prog_environ ML_lang Σ).
+  Notation "'WP' e {{ Φ } }" := (wp T ⊤ e%E Φ)
+    (at level 20, e, Φ at level 200, only parsing) : bi_scope.
+  Notation "'WP' e {{ v , Q } }" := (wp T ⊤ e%E (λ v, Q))
+    (at level 20, e, Q at level 200,
+     format "'[hv' 'WP'  e  '/' {{  '[' v ,  '/' Q  ']' } } ']'") : bi_scope.
+  Notation of_val w := (of_val ML_lang w%V).
+
+
+  Program Definition env_lookup (x : nat) : listO D -n> D :=
+    λne Δ, PersPred (default (inhabitant : persistent_pred _ _) (Δ !! x)).
+  Solve Obligations with repeat intros ?; simpl; solve_proper.
+
+  Definition interp_unit : listO D -n> D := λne Δ, PersPred (λ w, ⌜w = #LitUnit⌝)%I.
+  Definition interp_nat : listO D -n> D :=
+    λne Δ, PersPred (λ w, ⌜∃ (n:Z), w = # n⌝)%I.
+  Definition interp_bool : listO D -n> D :=
+    λne Δ, PersPred (λ w, ⌜∃ (b:bool), w = # b⌝)%I.
+
+  Program Definition interp_prod
+          (interp1 interp2 : listO D -n> D) : listO D -n> D :=
+    λne Δ,
+    PersPred (λ w, ∃ w1 w2, ⌜w = PairV w1 w2⌝ ∧ interp1 Δ w1 ∧ interp2 Δ w2)%I.
+  Solve Obligations with repeat intros ?; simpl; solve_proper.
+
+  Program Definition interp_sum
+      (interp1 interp2 : listO D -n> D) : listO D -n> D :=
+    λne Δ,
+    PersPred (λ w, (∃ w1, ⌜w = InjLV w1⌝ ∧ interp1 Δ w1) ∨
+                 (∃ w2, ⌜w = InjRV w2⌝ ∧ interp2 Δ w2))%I.
+  Solve Obligations with repeat intros ?; simpl; solve_proper.
+
+  Program Definition interp_arrow
+      (interp1 interp2 : listO D -n> D) : listO D -n> D :=
+    λne Δ,
+    PersPred (λ w, □ ∀ v, interp1 Δ v →
+                        WP App (of_val w) (of_val v) {{ interp2 Δ }})%I.
+  Solve Obligations with repeat intros ?; simpl; solve_proper.
+
+  Program Definition interp_forall
+      (interp : listO D -n> D) : listO D -n> D :=
+    λne Δ,
+    PersPred (λ w, □ ∀ τi : D, WP TApp (of_val w) {{ interp (τi :: Δ) }})%I.
+  Solve Obligations with repeat intros ?; simpl; solve_proper.
+
+  Program Definition interp_exist (interp : listO D -n> D) : listO D -n> D :=
+    λne Δ, PersPred (λ w, ∃ (τi : D) v, ⌜w = PackV v⌝ ∗ interp (τi :: Δ) v)%I.
+  Solve Obligations with repeat intros ?; simpl; solve_proper.
+
+  Definition interp_rec1 (interp : listO D -n> D) (Δ : listO D) (τi : D) : D :=
+    PersPred (λ w, □ (∃ v, ⌜w = RollV v⌝ ∧ ▷ interp (τi :: Δ) v))%I.
+
+  Global Instance interp_rec1_contractive
+    (interp : listO D -n> D) (Δ : listO D) : Contractive (interp_rec1 interp Δ).
+  Proof. by solve_contractive. Qed.
+
+  Lemma fixpoint_interp_rec1_eq (interp : listO D -n> D) Δ x :
+    fixpoint (interp_rec1 interp Δ) x ≡
+    interp_rec1 interp Δ (fixpoint (interp_rec1 interp Δ)) x.
+  Proof. exact: (fixpoint_unfold (interp_rec1 interp Δ) x). Qed.
+
+  Program Definition interp_rec (interp : listO D -n> D) : listO D -n> D :=
+    λne Δ, fixpoint (interp_rec1 interp Δ).
+  Next Obligation.
+    intros interp n Δ1 Δ2 HΔ; apply fixpoint_ne => τi w. solve_proper.
+  Qed.
+
+  Program Definition interp_ref_inv (l : loc) : D -n> iPropO Σ := λne τi,
+    (∃ v, l ↦M v ∗ τi v)%I.
+  Solve Obligations with solve_proper.
+
+  Program Definition interp_ref (interp : listO D -n> D) : listO D -n> D :=
+    λne Δ,
+    PersPred (λ w, ∃ (l:loc), ⌜w = # l⌝ ∧
+                      inv (logN .@ l) (interp_ref_inv l (interp Δ)))%I.
+  Solve Obligations with solve_proper.
+
+  Fixpoint interp (τ : type) : listO D -n> D :=
+    match τ return _ with
+    | TUnit => interp_unit
+    | TNat => interp_nat
+    | TBool => interp_bool
+    | TProd τ1 τ2 => interp_prod (interp τ1) (interp τ2)
+    | TSum τ1 τ2 => interp_sum (interp τ1) (interp τ2)
+    | TArrow τ1 τ2 => interp_arrow (interp τ1) (interp τ2)
+    | TVar x => env_lookup x
+    | TForall τ' => interp_forall (interp τ')
+    | TExist τ' => interp_exist (interp τ')
+    | TRec τ' => interp_rec (interp τ')
+    | Tref τ' => interp_ref (interp τ')
+    end.
+  Notation "⟦ τ ⟧" := (interp τ).
+
+  Definition interp_env (Γ : gmap string type)
+      (Δ : listO D) (vs : gmap string val) : iProp Σ :=
+    ([∗ map] x↦τ;v ∈ Γ;vs, ⟦ τ ⟧ Δ v)%I.
+  Notation "⟦ Γ ⟧*" := (interp_env Γ).
+
+  Definition interp_prog_type (Δ : listO D) s (t : program_type) : program_specification := match t with FunType tl tr =>
+    (λ s' vv Φ, ⌜s = s'⌝ ∗ ([∗ list] k↦τ;v ∈ tl;vv, ⟦ τ ⟧ Δ v) ∗ (∀ vr, ⟦ tr ⟧ Δ vr -∗ Φ vr))%I end.
+
+  (* Compare with languag/wp_link.v
+     The difference between this and program_fulfills is that we allow axiomatically specified
+     functions to be well-typed. *)
+  Definition program_spec_satisfied
+    (Tshould : program_specification) : iProp Σ := 
+    □ ∀ s vv Φ, Tshould s vv Φ -∗ WP (of_class _ (ExprCall s vv)) {{v, Φ v}}.
+
+  Global Instance prog_spec_sat_pers Tshould : Persistent (program_spec_satisfied Tshould).
+  Proof. apply intuitionistically_persistent. Qed.
+
+  Definition interp_prog_env (p_types : gmap string program_type) (Δ : listO D) : iProp Σ :=
+    ([∗ map] s↦τ ∈ p_types, program_spec_satisfied (interp_prog_type Δ s τ))%I.
+
+  Global Instance interp_prog_env_pers p_types Δ : Persistent (interp_prog_env p_types Δ).
+  Proof. eapply big_sepM_persistent. intros k x; apply prog_spec_sat_pers. Qed.
+
+  Definition interp_expr (τ : type) (Δ : listO D) (e : expr ML_lang) : iProp Σ :=
+    WP e {{ ⟦ τ ⟧ Δ }}%I.
+
+  Global Instance interp_env_base_persistent Δ Γ vs :
+  TCForall Persistent (zip_with (λ τ, ⟦ τ ⟧ Δ) Γ vs).
+  Proof. revert vs; induction Γ => vs; destruct vs; constructor; apply _. Qed.
+  Global Instance interp_env_persistent Γ Δ vs : Persistent (⟦ Γ ⟧* Δ vs) := _.
+
+  Lemma interp_weaken Δ1 Π Δ2 τ :
+    ⟦ τ.[upn (length Δ1) (ren (+ length Π))] ⟧ (Δ1 ++ Π ++ Δ2)
+    ≡ ⟦ τ ⟧ (Δ1 ++ Δ2).
+  Proof.
+    revert Δ1 Π Δ2. induction τ=> Δ1 Π Δ2; simpl; auto; intros ?; simpl.
+    - by repeat (f_equiv; try match goal with IH : ∀ _, _ |- _ => by apply IH end).
+    - by repeat (f_equiv; try match goal with IH : ∀ _, _ |- _ => by apply IH end).
+    - by repeat (f_equiv; try match goal with IH : ∀ _, _ |- _ => by apply IH end).
+    - f_equiv.
+      apply fixpoint_proper=> τi w /=.
+      by repeat (f_equiv; try match goal with IH : ∀ _, _ |- _ => by apply (IH (_ :: _)) end).
+    - rewrite iter_up; destruct lt_dec as [Hl | Hl]; simpl.
+      { by rewrite !lookup_app_l. }
+      rewrite !lookup_app_r; [|lia ..]; do 3 f_equiv; lia.
+    - by repeat (f_equiv; try match goal with IH : ∀ _, _ |- _ => by apply (IH (_ :: _)) end).
+    - by repeat (f_equiv; try match goal with IH : ∀ _, _ |- _ => by apply (IH (_ :: _)) end).
+    - by repeat (f_equiv; try match goal with IH : ∀ _, _ |- _ => by apply IH end).
+  Qed.
+
+  Lemma interp_subst_up Δ1 Δ2 τ τ' :
+    ⟦ τ ⟧ (Δ1 ++ interp τ' Δ2 :: Δ2)
+    ≡ ⟦ τ.[upn (length Δ1) (τ' .: ids)] ⟧ (Δ1 ++ Δ2).
+  Proof.
+    revert Δ1 Δ2; induction τ=> Δ1 Δ2; simpl; auto; intros ?; simpl.
+    - by repeat (f_equiv; try match goal with IH : ∀ _, _ |- _ => by apply IH end).
+    - by repeat (f_equiv; try match goal with IH : ∀ _, _ |- _ => by apply IH end).
+    - by repeat (f_equiv; try match goal with IH : ∀ _, _ |- _ => by apply IH end).
+    - f_equiv.
+      apply fixpoint_proper=> τi w /=.
+      by repeat (f_equiv; try match goal with IH : ∀ _, _ |- _ => by apply (IH (_ :: _)) end).
+    - match goal with |- context [_ !! ?x] => rename x into idx end.
+      rewrite iter_up; destruct lt_dec as [Hl | Hl]; simpl.
+      { by rewrite !lookup_app_l. }
+      rewrite !lookup_app_r; [|lia ..].
+      case EQ: (idx - length Δ1) => [|n]; simpl.
+      { symmetry. asimpl. apply (interp_weaken [] Δ1 Δ2 τ'). }
+      rewrite !lookup_app_r; [|lia ..]. do 3 f_equiv. lia.
+    - by repeat (f_equiv; try match goal with IH : ∀ _, _ |- _ => by apply (IH (_ :: _)) end).
+    - by repeat (f_equiv; try match goal with IH : ∀ _, _ |- _ => by apply (IH (_ :: _)) end).
+    - by repeat (f_equiv; try match goal with IH : ∀ _, _ |- _ => by apply IH end).
+  Qed.
+
+  Lemma interp_subst Δ2 τ τ' v : ⟦ τ ⟧ (⟦ τ' ⟧ Δ2 :: Δ2) v ≡ ⟦ τ.[τ'/] ⟧ Δ2 v.
+  Proof. apply (interp_subst_up []). Qed.
+
+  Lemma interp_env_dom Δ Γ vs : ⟦ Γ ⟧* Δ vs ⊢ ⌜dom Γ = dom vs⌝.
+  Proof. iIntros "H". by iApply big_sepM2_dom. Qed.
+
+  Lemma interp_env_Some_l Δ Γ vs x τ :
+    Γ !! x = Some τ → ⟦ Γ ⟧* Δ vs ⊢ ∃ v, ⌜vs !! x = Some v⌝ ∧ ⟦ τ ⟧ Δ v.
+  Proof.
+    iIntros (?) "HΓ". iAssert (⌜x ∈ dom vs⌝)%I as "%HH".
+    1: { iPoseProof (interp_env_dom with "HΓ") as "<-". iPureIntro. by eapply elem_of_dom_2. }
+    revert HH; intros [v Hv]%elem_of_dom.
+    iExists v; iSplitR; first done.
+    iPoseProof (big_sepM2_lookup with "HΓ") as "HΓ". 1-2: done. done.
+  Qed.
+
+  Lemma interp_env_nil Δ : ⊢ ⟦ ∅ ⟧* Δ ∅.
+  Proof. iApply big_sepM2_empty. done. Qed.
+  Lemma interp_env_insert Δ Γ vs τ v x :
+    Γ !! x = None → vs !! x = None →
+    (⟦ <[x:=τ]> Γ ⟧* Δ ( <[x:=v]> vs) ⊣⊢ ⟦ τ ⟧ Δ v ∗ ⟦ Γ ⟧* Δ vs).
+  Proof.
+    intros H1 H2. iApply big_sepM2_insert; done.
+  Qed.
+
+  Lemma interp_env_ren Δ (Γ : gmap string type) (vs : gmap string val) τi :
+    ⟦ subst (ren (+1)) <$> Γ ⟧* (τi :: Δ) vs ⊣⊢ ⟦ Γ ⟧* Δ vs.
+  Proof.
+    iStartProof.
+    iSplit; iIntros "H";
+    iPoseProof (interp_env_dom with "H") as "%Hdom".
+    all: try rewrite dom_fmap_L in Hdom.
+    all: (iPoseProof big_sepM2_fmap_l as "[HL HR]").
+    - iPoseProof ("HL" with "H") as "H". iClear "HL HR".
+      iApply (big_sepM2_wand with "H"). iApply big_sepM2_intro.
+      1: intros k; erewrite <- !elem_of_dom, Hdom; done.
+      iIntros "!> %k %τ %v %H1 %H2 H". iPoseProof (interp_weaken [] [τi] Δ with "H") as "H". done.
+    - iApply "HR"; iClear "HL HR".
+      iApply (big_sepM2_wand with "H"). iApply big_sepM2_intro.
+      1: intros k; erewrite <- !elem_of_dom, Hdom; done.
+      iIntros "!> %k %τ %v %H1 %H2 H". iApply (interp_weaken [] [τi] Δ). done.
+  Qed.
+End logrel.
+
+Global Typeclasses Opaque interp_env.
+
+Notation "⟦ P ⟧ₚ*  x" := (interp_prog_env x P) (at level 10).
+Notation "⟦ τ ⟧  x" := (interp x τ) (at level 10).
+Notation "⟦ τ ⟧ₑ  x" := (interp_expr x τ) (at level 10).
+Notation "⟦ Γ ⟧*  x" := (interp_env x Γ) (at level 10).
+
