theories/ml_toy_lang/logrel/typing.v
@@ -1,0 +1,182 @@
+From melocoton.ml_toy_lang Require Export lang notation metatheory.
+From Autosubst Require Import Autosubst.
+From iris.prelude Require Import options.
+
+Inductive type :=
+  | TUnit : type
+  | TNat : type
+  | TBool : type
+  | TProd : type → type → type
+  | TSum : type → type → type
+  | TArrow : type → type → type
+  | TRec (τ : {bind 1 of type})
+  | TVar (x : var)
+  | TForall (τ : {bind 1 of type})
+  | TExist (τ : {bind 1 of type})
+  | Tref (τ : type). (* References are length one. Handling dynamic arrays is difficult *)
+
+Global Instance Ids_type : Ids type. derive. Defined.
+Global Instance Rename_type : Rename type. derive. Defined.
+Global Instance Subst_type : Subst type. derive. Defined.
+Global Instance SubstLemmas_typer : SubstLemmas type. derive. Qed.
+
+Definition binop_arithmetic (op : bin_op) : bool :=
+  match op with
+  | PlusOp | MinusOp| MultOp| QuotOp| RemOp| AndOp| OrOp| XorOp| ShiftLOp| ShiftROp => true
+  | LeOp| LtOp| EqOp => false
+  end.
+
+Definition binop_arithmetic_to_bool (op : bin_op) : bool :=
+  match op with
+  | PlusOp | MinusOp| MultOp| QuotOp| RemOp| AndOp| OrOp| XorOp| ShiftLOp| ShiftROp | EqOp => false
+  | LeOp| LtOp => true
+  end.
+
+Definition binop_boolish (op : bin_op) : bool :=
+  match op with
+  | AndOp| OrOp| XorOp => true
+  | _ => false
+  end.
+
+Inductive EqType : type → Prop :=
+  | EqTUnit : EqType TUnit
+  | EqTNat : EqType TNat
+  | EqTBool : EqType TBool
+  | EQRef τ : EqType (Tref τ).
+
+
+Inductive program_type := FunType : list type -> type -> program_type.
+Definition program_env := gmap string program_type.
+
+Section IndDef.
+Context (P : program_env).
+
+Reserved Notation "Γ ⊢ₜ e : τ" (at level 74, e, τ at next level).
+Unset Elimination Schemes.
+Inductive typed (Γ : gmap string type) : expr → type → Prop :=
+  | Var_typed x τ : Γ !! x = Some τ → Γ ⊢ₜ Var x : τ 
+  | Unit_typed : Γ ⊢ₜ  #LitUnit : TUnit
+  | Nat_typed (n:Z) : Γ ⊢ₜ # n : TNat
+  | Bool_typed (b:bool) : Γ ⊢ₜ # b : TBool
+  | BinOp_typed_nat_nat op e1 e2 :
+     binop_arithmetic op = true → 
+     Γ ⊢ₜ e1 : TNat → Γ ⊢ₜ e2 : TNat → Γ ⊢ₜ BinOp op e1 e2 : TNat
+  | BinOp_typed_nat_bool op e1 e2 :
+     binop_arithmetic_to_bool op = true → 
+     Γ ⊢ₜ e1 : TNat → Γ ⊢ₜ e2 : TNat → Γ ⊢ₜ BinOp op e1 e2 : TBool
+  | BinOp_typed_bool op e1 e2 :
+     binop_boolish op = true → 
+     Γ ⊢ₜ e1 : TBool → Γ ⊢ₜ e2 : TBool → Γ ⊢ₜ BinOp op e1 e2 : TBool
+  | BinOp_typed_eq T op e1 e2 :
+     EqType T → 
+     Γ ⊢ₜ e1 : T → Γ ⊢ₜ e2 : T → Γ ⊢ₜ BinOp op e1 e2 : TBool
+  | Pair_typed e1 e2 τ1 τ2 : Γ ⊢ₜ e1 : τ1 → Γ ⊢ₜ e2 : τ2 → Γ ⊢ₜ Pair e1 e2 : TProd τ1 τ2
+  | Fst_typed e τ1 τ2 : Γ ⊢ₜ e : TProd τ1 τ2 → Γ ⊢ₜ Fst e : τ1
+  | Snd_typed e τ1 τ2 : Γ ⊢ₜ e : TProd τ1 τ2 → Γ ⊢ₜ Snd e : τ2
+  | InjL_typed e τ1 τ2 : Γ ⊢ₜ e : τ1 → Γ ⊢ₜ InjL e : TSum τ1 τ2
+  | InjR_typed e τ1 τ2 : Γ ⊢ₜ e : τ2 → Γ ⊢ₜ InjR e : TSum τ1 τ2
+  | Case_typed e0 e1 e2 τ1 τ2 τ3 :
+     Γ ⊢ₜ e0 : TSum τ1 τ2 → Γ ⊢ₜ e1 : (TArrow τ1 τ3) → Γ ⊢ₜ e2 : (TArrow τ2 τ3) →
+     Γ ⊢ₜ Case e0 e1 e2 : τ3
+  | If_typed e0 e1 e2 τ :
+     Γ ⊢ₜ e0 : TBool → Γ ⊢ₜ e1 : τ → Γ ⊢ₜ e2 : τ → Γ ⊢ₜ If e0 e1 e2 : τ
+  | Rec_typed f x e τ1 τ2 :
+     (binder_insert f (TArrow τ1 τ2) (binder_insert x τ1 Γ)) ⊢ₜ e : τ2 → Γ ⊢ₜ Rec f x e : TArrow τ1 τ2
+  | App_typed e1 e2 τ1 τ2 :
+     Γ ⊢ₜ e1 : TArrow τ1 τ2 → Γ ⊢ₜ e2 : τ1 → Γ ⊢ₜ App e1 e2 : τ2
+  | TLam_typed e τ :
+     subst (ren (+1)) <$> Γ ⊢ₜ e : τ → Γ ⊢ₜ TLam e : TForall τ
+  | TApp_typed e τ τ' : Γ ⊢ₜ e : TForall τ → Γ ⊢ₜ TApp e : τ.[τ'/]
+  | Pack_typed e τ τ' :
+     Γ ⊢ₜ e : τ.[τ'/] → Γ ⊢ₜ Pack e : TExist τ
+  | UnpackIn_typed x e1 e2 τ τ' :
+     Γ ⊢ₜ e1 : TExist τ →
+     binder_insert x τ (subst (ren (+1)) <$> Γ) ⊢ₜ e2 : τ'.[ren (+1)] →
+     Γ ⊢ₜ UnpackIn x e1 e2 : τ'
+  | TRoll e τ : Γ ⊢ₜ e : τ.[TRec τ/] → Γ ⊢ₜ Roll e : TRec τ
+  | TUnroll e τ : Γ ⊢ₜ e : TRec τ → Γ ⊢ₜ Unroll e : τ.[TRec τ/] 
+  | TAlloc e τ : Γ ⊢ₜ e : τ → Γ ⊢ₜ Alloc e (#1) : Tref τ 
+  | TLoad e τ : Γ ⊢ₜ e : Tref τ → Γ ⊢ₜ Load e #0 : τ 
+  | TStore e e' τ : Γ ⊢ₜ e : Tref τ → Γ ⊢ₜ e' : τ → Γ ⊢ₜ Store e (#0) e' : TUnit 
+  | TExtern s el tl tr :
+      P !! s = Some (FunType tl tr) →
+      Forall2 (typed Γ) el tl →
+      Γ ⊢ₜ (Extern s el) : tr (*
+  | TCAS e1 e2 e3 τ :
+     EqType τ → Γ ⊢ₜ e1 : Tref τ → Γ ⊢ₜ e2 : τ → Γ ⊢ₜ e3 : τ →
+     Γ ⊢ₜ CAS e1 e2 e3 : TBool
+  | TFAA e1 e2 : Γ ⊢ₜ e1 : Tref TNat → Γ ⊢ₜ e2 : TNat → Γ ⊢ₜ FAA e1 e2 : TNat *)
+where "Γ ⊢ₜ e : τ" := (typed Γ e τ).
+
+(* Forall2 (typed Γ) requires special care *)
+Lemma typed_ind (P0 : gmap string type → expr → type → Prop) : 
+  (∀ (Γ : gmap string type) (x : string) (τ : type), Γ !! x = Some τ → P0 Γ x τ)
+→ (∀  Γ : gmap string type, P0 Γ #() TUnit)
+→ (∀ (Γ : gmap string type) (n : Z), P0 Γ #n TNat)
+→ (∀ (Γ : gmap string type) (b : bool), P0 Γ #b TBool)
+→ (∀ (Γ : gmap string type) (op : bin_op) (e1 e2 : expr), binop_arithmetic op = true → Γ ⊢ₜ e1 : TNat → P0 Γ e1 TNat → Γ ⊢ₜ e2 : TNat → P0 Γ e2 TNat → P0 Γ (BinOp op e1 e2) TNat)
+→ (∀ (Γ : gmap string type) (op : bin_op) (e1 e2 : expr), binop_arithmetic_to_bool op = true → Γ ⊢ₜ e1 : TNat → P0 Γ e1 TNat → Γ ⊢ₜ e2 : TNat → P0 Γ e2 TNat → P0 Γ (BinOp op e1 e2) TBool)
+→ (∀ (Γ : gmap string type) (op : bin_op) (e1 e2 : expr), binop_boolish op = true → Γ ⊢ₜ e1 : TBool → P0 Γ e1 TBool → Γ ⊢ₜ e2 : TBool → P0 Γ e2 TBool → P0 Γ (BinOp op e1 e2) TBool)
+→ (∀ (Γ : gmap string type) (T : type) (op : bin_op) (e1 e2 : expr), EqType T → Γ ⊢ₜ e1 : T → P0 Γ e1 T → Γ ⊢ₜ e2 : T → P0 Γ e2 T → P0 Γ (BinOp op e1 e2) TBool)
+→ (∀ (Γ : gmap string type) (e1 e2 : expr) (τ1 τ2 : type), Γ ⊢ₜ e1 : τ1 → P0 Γ e1 τ1 → Γ ⊢ₜ e2 : τ2 → P0 Γ e2 τ2 → P0 Γ (e1, e2)%E (TProd τ1 τ2))
+→ (∀ (Γ : gmap string type) (e : expr) (τ1 τ2 : type), Γ ⊢ₜ e : TProd τ1 τ2 → P0 Γ e (TProd τ1 τ2) → P0 Γ (Fst e) τ1)
+→ (∀ (Γ : gmap string type) (e : expr) (τ1 τ2 : type), Γ ⊢ₜ e : TProd τ1 τ2 → P0 Γ e (TProd τ1 τ2) → P0 Γ (Snd e) τ2)
+→ (∀ (Γ : gmap string type) (e : expr) (τ1 τ2 : type), Γ ⊢ₜ e : τ1 → P0 Γ e τ1 → P0 Γ (InjL e) (TSum τ1 τ2))
+→ (∀ (Γ : gmap string type) (e : expr) (τ1 τ2 : type), Γ ⊢ₜ e : τ2 → P0 Γ e τ2 → P0 Γ (InjR e) (TSum τ1 τ2))
+→ (∀ (Γ : gmap string type) (e0 e1 e2 : expr) (τ1 τ2 τ3 : type), Γ ⊢ₜ e0 : TSum τ1 τ2 → P0 Γ e0 (TSum τ1 τ2) → Γ ⊢ₜ e1 : TArrow τ1 τ3 → P0 Γ e1 (TArrow τ1 τ3) → Γ ⊢ₜ e2 : TArrow τ2 τ3 → P0 Γ e2 (TArrow τ2 τ3) → P0 Γ (Case e0 e1 e2) τ3)
+→ (∀ (Γ : gmap string type) (e0 e1 e2 : expr) (τ : type), Γ ⊢ₜ e0 : TBool → P0 Γ e0 TBool → Γ ⊢ₜ e1 : τ → P0 Γ e1 τ → Γ ⊢ₜ e2 : τ → P0 Γ e2 τ → P0 Γ (if: e0 then e1 else e2)%E τ)
+→ (∀ (Γ : gmap string type) (f14 x : binder) (e : expr) (τ1 τ2 : type), binder_insert f14 (TArrow τ1 τ2) (binder_insert x τ1 Γ) ⊢ₜ e : τ2 → P0 (binder_insert f14 (TArrow τ1 τ2) (binder_insert x τ1 Γ)) e τ2 → P0 Γ (rec: f14 x := e)%E (TArrow τ1 τ2))
+→ (∀ (Γ : gmap string type) (e1 e2 : expr) (τ1 τ2 : type), Γ ⊢ₜ e1 : TArrow τ1 τ2 → P0 Γ e1 (TArrow τ1 τ2) → Γ ⊢ₜ e2 : τ1 → P0 Γ e2 τ1 → P0 Γ (e1 e2) τ2)
+→ (∀ (Γ : gmap string type) (e : expr) (τ : type), subst (ren (+1)) <$> Γ ⊢ₜ e : τ → P0 (subst (ren (+1)) <$> Γ) e τ → P0 Γ (Λ: <>, e)%E (TForall τ))
+→ (∀ (Γ : gmap string type) (e : expr) (τ τ' : {bind type}), Γ ⊢ₜ e : TForall τ → P0 Γ e (TForall τ) → P0 Γ (TApp e) τ.[τ'/])
+→ (∀ (Γ : gmap string type) (e : expr) (τ τ' : type), Γ ⊢ₜ e : τ.[τ'/] → P0 Γ e τ.[τ'/] → P0 Γ (pack:e)%E (TExist τ))
+→ (∀ (Γ : gmap string type) (x : binder) (e1 e2 : expr) (τ : {bind type}) (τ' : type),
+Γ ⊢ₜ e1 : TExist τ → P0 Γ e1 (TExist τ) → binder_insert x τ (subst (ren (+1)) <$> Γ) ⊢ₜ e2 : τ'.[ren (+1)] → P0 (binder_insert x τ (subst (ren (+1)) <$> Γ)) e2 τ'.[ren (+1)] → P0 Γ (unpack: x := e2 in e1)%E τ')
+→ (∀ (Γ : gmap string type) (e : expr) (τ : {bind type}), Γ ⊢ₜ e : τ.[TRec τ/] → P0 Γ e τ.[TRec τ/] → P0 Γ (roll:e)%E (TRec τ))
+→ (∀ (Γ : gmap string type) (e : expr) (τ : {bind type}), Γ ⊢ₜ e : TRec τ → P0 Γ e (TRec τ) → P0 Γ (unroll:e)%E τ.[TRec τ/])
+→ (∀ (Γ : gmap string type) (e : expr) (τ : type), Γ ⊢ₜ e : τ → P0 Γ e τ → P0 Γ ((ref e)%E #1) (Tref τ))
+→ (∀ (Γ : gmap string type) (e : expr) (τ : type), Γ ⊢ₜ e : Tref τ → P0 Γ e (Tref τ) → P0 Γ ((! e)%E #0) τ)
+→ (∀ (Γ : gmap string type) (e e' : expr) (τ : type), Γ ⊢ₜ e : Tref τ → P0 Γ e (Tref τ) → Γ ⊢ₜ e' : τ → P0 Γ e' τ → P0 Γ ((e <- #0)%E e') TUnit)
+→ (∀ (Γ : gmap string type) (s : string) (el : list expr) (tl : list type) (tr : type),
+       P !! s = Some (FunType tl tr) → Forall2 (P0 Γ) el tl → P0 Γ (Extern s el) tr) → ∀ (Γ : gmap string type) (e : expr) (t : type), Γ ⊢ₜ e : t → P0 Γ e t.
+Proof.
+  do 27 intros ?.
+  fix IH 4. intros ???; destruct 1; try eauto.
+  enough (Forall2 (P0 Γ) el tl) by eauto.
+  clear H26.
+  revert el tl H27. fix IHf 3.
+  intros el tl; destruct 1; econstructor.
+  1: by eapply IH.
+  by eapply IHf.
+Qed.
+
+Definition env_subst := subst_all.
+
+Lemma env_subst_lookup vs x v :
+  vs !! x = Some v → env_subst vs (Var x) = of_val v.
+Proof.
+  intros H. cbn. rewrite H. done.
+Qed.
+
+Lemma typed_closed Γ τ e : Γ ⊢ₜ e : τ → is_closed_expr (dom Γ) e.
+Proof.
+  intros H; induction H using typed_ind; cbn; eauto.
+  - by eapply bool_decide_pack, elem_of_dom_2.
+  - by rewrite !dom_binder_insert in IHtyped.
+  - by erewrite dom_fmap_L in IHtyped.
+  - eapply andb_prop_intro; split; eauto.
+    eapply bool_decide_pack; set_solver.
+  - rewrite !dom_binder_insert !dom_fmap_L in IHtyped2. eauto.
+  - eapply andb_prop_intro; split; eauto.
+    eapply bool_decide_pack; set_solver.
+  - eapply andb_prop_intro; split; eauto.
+    eapply bool_decide_pack; set_solver.
+  - eauto 10.
+  - eapply forallb_True, Forall2_Forall_l. 1:done.
+    eapply Forall_true. done.
+Qed.
+Set Elimination Schemes.
+End IndDef.
+
+
+Notation "P ; Γ ⊢ₜ e : τ" := (typed P Γ e τ) (at level 74, e, τ at next level).
